thy/OpenFlow/LinuxRouterOpenFlowTranslation.thy
@@ -1,5 +1,5 @@
 theory LinuxRouterOpenFlowTranslation
-imports 
+imports "../IP_Addresses/CIDR_Split"
   "../Automaticc_Refinement/Misc" (*TODO@Peter: rename and make available at better place :)*)
 	"../Simple_Firewall/Generic_SimpleFw" 
 	"Semantics_OpenFlow"
