thy/Simple_Firewall/Common/SetPartitioning.thy
@@ -4,7 +4,13 @@ imports Main
 begin
 
 section\<open>Partition a set by a specifc constraint\<close>
-text\<open>Will be used for the IP address space partition of a firewall. This file is completely generic.\<close>
+text\<open>Will be used for the IP address space partition of a firewall.
+    However, this file is completely generic in terms of sets, it only imports Main.
+
+    It will be used in @{file "../Service_Matrices.thy"}.
+    Core idea: This file partitions @{typ "'a set set"} by some magic condition.
+    Later, we will show that this magic condition implies that all IPs that have been grouped
+    by the magic condition show the same behaviour for a simple firewall.\<close>
 
 (* disjoint, ipPartition definitions *)
 
